examples/low-level/crypto/Crypto.Symmetric.Poly1305.MAC.fst
@@ -113,12 +113,15 @@ noeq type state (i:id) =
 let genPost0 (i:id) (region:rid{is_eternal_region region}) m0 (st: state i) m1 =
     ~(contains m0 st.r) /\
     ~(contains m0 st.s) /\
-    modifies (Set.singleton region) m0 m1 /\ 
     st.region == region /\
-    (mac_log ==> m_contains (ilog st.log) m1 /\ m_sel m1 (ilog st.log) == None)
+    (mac_log ==> 
+        ~ (m_contains (ilog st.log) m0) /\ 
+	   m_contains (ilog st.log) m1 /\ 
+	   m_sel m1 (ilog st.log) == None)
 
 let genPost (i:id) (region:rid{is_eternal_region region}) m0 (st: state i) m1 =
     genPost0 i region m0 st m1 /\
+    modifies (Set.singleton region) m0 m1 /\ 
     modifies_rref region TSet.empty m0.h m1.h 
 
 val alloc: i:id
